prove  back_reachable_twoPC  and reachable_twoPC with a set s of unreachable state

Star/BackwardsInvariants/TwoPhaseCommit.lean
@@ -47,6 +47,11 @@ theorem φ_backwards_reachable_iff {T} {l : LTS T} {s} :
   l.φ s ↔ (∃ s_init, l.flushed s_init ∧ l.backwards_reachable_from s_init s) := by
   grind [backwards_reachable_φ, φ_backwards_reachable]
 
+theorem φ_reachable_iff {T} {l : LTS T} {s} :
+  l.φ s ↔ l.reachable s := by admit
+  grind [φ_backwards_reachable_iff, LTS.reachable]
+
+
 namespace TEST
 
 def test : LTS (Fin 3) where
@@ -66,7 +71,7 @@ theorem reachable : test.reachable (20:Nat) := by
   · apply ReflTransGen.single; exists 0
   · apply ReflTransGen.single; exists 1
 
-theorem back_reachable {x} : test.backwards_reachable_from (30:Nat) x → x ≠ (0:Nat) := by
+theorem back_reachable {x} : test.backwards_reachable_from (30:Nat) x → x = (30:Nat) := by
   dsimp [LTS.backwards_reachable_from]
   intro h
   generalize h30 : 30 = x30 at h
@@ -96,7 +101,6 @@ theorem back_reachable3 : test.backwards_reachable_from (20:Nat) (0:Nat) := by
 
 end TEST
 
-end THEORY
 
 namespace TwoPhaseCommit
 
@@ -120,6 +124,7 @@ def PState.consistentWith (b : Bool) : PState → Bool
 | .committed b' => b == b'
 | .aborted => true
 
+
 structure State where
   p12c : Option Bool
   p22c : Option Bool
@@ -140,7 +145,8 @@ inductive Protocol : Rule → State → State → Prop where
 | step_part1 {s : State} {b : Bool} : s.p1 = .tentative b → Protocol .part1 s {s with p12c := .some b}
 | step_part2 {s : State} {b : Bool} : s.p2 = .tentative b → Protocol .part2 s {s with p22c := .some b}
 | step_commit {s : State} : s.p12c.isSome → s.p12c = s.p22c → Protocol .commit s {p1 := s.p1.commit, p2 := s.p2.commit, p12c := .none, p22c := .none}
-| step_abort {s : State} : s.p12c.isSome → s.p12c.isSome → s.p12c ≠ s.p22c → Protocol .abort s {s with p1 := s.p1.abort, p2 := s.p2.abort, p12c := .none, p22c := .none}
+--| step_abort {s : State} : s.p12c.isSome → s.p12c.isSome → s.p12c ≠ s.p22c → Protocol .abort s {s with p1 := s.p1.abort, p2 := s.p2.abort, p12c := .none, p22c := .none}
+
 
 inductive φ : State → Prop where
 | base_commit {b : Bool}:
@@ -149,6 +155,201 @@ inductive φ : State → Prop where
   φ {p1 := .aborted, p2 := .aborted, p12c := .none, p22c := .none}
 | step {s s' : State} {r : Rule}:
   φ s' → Protocol r s s' → φ s
+
+
+def init : State → Prop :=
+  fun s => s.p1 = .empty ∧ s.p2 = .empty ∧ s.p12c.isNone ∧ s.p22c.isNone
+
+
+
+def init_state : State  := {
+  p1 := .empty
+  p2 := .empty
+  p12c := none
+  p22c := none
+}
+
+
+
+-- Define LTS for the two-phase commit protocol
+def twoPC : LTS Rule where
+  S := State
+  transitions := Protocol
+  init s := init s
+  flushed s := φ s
+
+def unreachable_set (s : State) : Prop :=
+  ∃ b, (s.p1 = .tentative b ∧ s.p12c = some (!b)) ∨ (s.p2 = .tentative b ∧ s.p22c = some (!b))
+
+
+theorem back_reachable_twoPC {x} : ∀ s, unreachable_set s -> twoPC.backwards_reachable_from s x → unreachable_set x := by
+  dsimp [LTS.backwards_reachable_from]
+  intro s hu h
+  induction h using ReflTransGen.head_induction_on with
+  | refl => grind
+  | @head a c h1 h2 h3 =>
+    clear h2
+    dsimp [Function.swap, twoPC, LTS.atrans] at h1
+    obtain ⟨t, ht⟩ := h1
+    cases t
+    . cases ht
+      simp_all
+      unfold unreachable_set at hu
+      cases hu; rename_i H
+      cases H
+      . simp_all
+      . apply h3
+        unfold unreachable_set at *
+        simp_all
+    . cases ht
+      simp_all
+      unfold unreachable_set at hu
+      cases hu; rename_i H
+      cases H
+      . apply h3
+        unfold unreachable_set at *
+        simp_all
+      . simp_all
+    . cases ht
+      simp_all
+      unfold unreachable_set at hu
+      cases hu; rename_i H
+      cases H
+      . grind
+      . apply h3
+        unfold unreachable_set at *
+        simp_all
+    . cases ht
+      simp_all
+      unfold unreachable_set at hu
+      cases hu; rename_i H
+      cases H
+      . apply h3
+        unfold unreachable_set at *
+        simp_all
+      . grind
+    . cases ht
+      simp_all
+      unfold unreachable_set at hu
+      cases hu; rename_i H
+      cases H
+      . grind
+      . apply h3
+        unfold unreachable_set at *
+        simp_all
+    . cases ht
+
+
+theorem reachable_twoPC : ∀ s, unreachable_set s -> ¬ twoPC.reachable s := by
+  intro s h hreach
+  dsimp [LTS.reachable] at hreach
+  specialize hreach _
+  . exact init_state
+  . specialize hreach (by unfold init_state; constructor; simp_all; grind)
+    rw [Relation.reflTransGen_swap] at hreach
+    have h' := back_reachable_twoPC _ h hreach
+    unfold unreachable_set at *
+    unfold init_state at *
+    simp_all
+
+def test_state : State  := {
+  p1 := .tentative true
+  p2 := .empty
+  p12c := false
+  p22c := none
+}
+
+def test_state1 : State  := {
+  p1 := .tentative false
+  p2 := .empty
+  p12c := true
+  p22c := none
+}
+
+def test_state2 : State  := {
+  p1 := .empty
+  p2 := .tentative false
+  p12c := none
+  p22c := true
+}
+
+def test_state3 : State  := {
+  p1 := .empty
+  p2 := .tentative true
+  p12c := none
+  p22c := false
+}
+
+def test_state4 : State  := {
+  p1 := .empty
+  p2 := .tentative true
+  p12c := none
+  p22c := true
+}
+
+
+
+theorem reachable_twoPC_test : ¬ twoPC.reachable test_state := by
+  intro hreach
+  dsimp [LTS.reachable] at hreach
+  specialize hreach _
+  . exact init_state
+  . specialize hreach (by unfold init_state; constructor; simp_all; grind)
+    rw [Relation.reflTransGen_swap] at hreach
+    have h' := back_reachable_twoPC _ (by unfold unreachable_set; unfold test_state; simp_all) hreach
+    unfold unreachable_set at *
+    unfold init_state at *
+    simp_all
+
+theorem reachable_twoPC_test1 : ¬ twoPC.reachable test_state1 := by
+  intro hreach
+  dsimp [LTS.reachable] at hreach
+  specialize hreach _
+  . exact init_state
+  . specialize hreach (by unfold init_state; constructor; simp_all; grind)
+    rw [Relation.reflTransGen_swap] at hreach
+    have h' := back_reachable_twoPC _ (by unfold unreachable_set; unfold test_state1; simp_all) hreach
+    unfold unreachable_set at *
+    unfold init_state at *
+    simp_all
+
+theorem reachable_twoPC_test2 : ¬ twoPC.reachable test_state2 := by
+  intro hreach
+  dsimp [LTS.reachable] at hreach
+  specialize hreach _
+  . exact init_state
+  . specialize hreach (by unfold init_state; constructor; simp_all; grind)
+    rw [Relation.reflTransGen_swap] at hreach
+    have h' := back_reachable_twoPC _ (by unfold unreachable_set; unfold test_state2; simp_all) hreach
+    unfold unreachable_set at *
+    unfold init_state at *
+    simp_all
+
+theorem reachable_twoPC_test3 : ¬ twoPC.reachable test_state3 := by
+  intro hreach
+  dsimp [LTS.reachable] at hreach
+  specialize hreach _
+  . exact init_state
+  . specialize hreach (by unfold init_state; constructor; simp_all; grind)
+    rw [Relation.reflTransGen_swap] at hreach
+    have h' := back_reachable_twoPC _ (by unfold unreachable_set; unfold test_state3; simp_all) hreach
+    unfold unreachable_set at *
+    unfold init_state at *
+    simp_all
+
+
+-- theorem reachable_twoPC_test4 : ¬ twoPC.reachable test_state4 := by
+--   intro hreach
+--   dsimp [LTS.reachable] at hreach
+--   specialize hreach _
+--   . exact init_state
+--   . specialize hreach (by unfold init_state; constructor; simp_all; grind)
+--     rw [Relation.reflTransGen_swap] at hreach
+--     have h' := back_reachable_twoPC _ (by unfold unreachable_set; unfold test_state4; simp_all) hreach
+--     unfold unreachable_set at *
+--     unfold init_state at *
+--     simp_all
+
 
 theorem comm_pinit1_pinit2 {s s' s''} :
   Protocol .pinit1 s s' →
@@ -234,71 +435,91 @@ theorem comm_pinit2_commit {s s' s''} :
     cases h₂ with
     | step_commit hs heq => simp_all
 
+
+--should be easy
 theorem part1_det {s s' s''} :
   Protocol .part1 s s' →
   Protocol .part1 s s'' →
-  s' = s'' := by sorry
+  s' = s'' := by
+  intro h1 h2;
+  cases h1 ; cases h2 ; grind
 
-theorem part1_twice {s s'} :
-  Protocol .part1 s s' →
-  Protocol .part1 s' s' := by sorry
-
-theorem comm_part1_commit' {s b} (hphi : φ s) :
-  s.p12c = .some b ∧ s.p1.consistentWith b := by
-  induction hphi generalizing b with
-  | base_commit => sorry
-  | base_abort => sorry
-  | @step s_p s'_p r hphi' hprot ih =>
-    cases r with
-    | pinit1 =>
-      cases hprot; grind
-    | pinit2 =>
-      cases hprot; grind
-    | part2 =>
-      cases hprot; grind
-    | part1 =>
-      cases hprot; specialize @ih b
-      dsimp [PState.consistentWith] at *
-      rename_i a
-      rw [a] at ih ⊢; dsimp at *
-
-    | commit =>
-      cases hprot; specialize @ih true; grind
-    | abort =>
-      cases hprot; specialize @ih true; grind
 
 theorem comm_part1_commit {s s' s''} (hphi : φ s) :
-  Protocol .part1 s s' →
-  Protocol .commit s s'' →
-  Protocol .commit s' s'' := by
-  induction hphi generalizing s' s'' with
-  | base_commit => sorry
-  | base_abort => sorry
-  | @step s_p s'_p r hphi' hprot ih =>
-    intro htrans1 htrans2
-    cases r with
-    | pinit1 =>
-      obtain ⟨s_pinit_comm, h_pinit, h_comm⟩ := comm_pinit1_commit ‹_› ‹_›
-      obtain ⟨s_pinit_part1, h_pinit2, h_part1⟩ := comm_pinit1_part1 hprot ‹_›
-      have : Protocol Rule.commit s_pinit_part1 s_pinit_comm := by grind
-      sorry
-    | pinit2 =>
-      sorry
-    | part2 =>
-      sorry
-    | part1 =>
-      have : s'_p = s' := by grind [part1_det]
-      subst_vars
-      apply ih; grind [part1_twice]
-      skip
-    | commit => sorry
-    | abort => sorry
+  twoPC.φ s →
+  twoPC.transitions .part1 s s' →
+  twoPC.transitions .commit s s'' →
+  twoPC.transitions .commit s' s'' := by
+  intro h1 h2 h3
+  have H := @φ_backwards_reachable_iff _ twoPC s
+  rcases H with ⟨ H, H1⟩
+  specialize H h1
 
-theorem comm_part2_commit {s s' s''} :
-  Protocol .part2 s s' →
-  Protocol .commit s s'' →
-  ∃ s''', Protocol .part2 s'' s''' ∧ Protocol .commit s' s''' := by
-  -- Commit makes p2 committed, disabling the part2 step on that branch.
-  sorry
+
+
+-- theorem part1_twice {s s'} :
+--   Protocol .part1 s s' →
+--   Protocol .part1 s' s' := by sorry
+
+-- theorem comm_part1_commit' {s b} (hphi : φ s) :
+--   s.p12c = .some b ∧ s.p1.consistentWith b := by
+--   induction hphi generalizing b with
+--   | base_commit => sorry
+--   | base_abort => sorry
+--   | @step s_p s'_p r hphi' hprot ih =>
+--     cases r with
+--     | pinit1 =>
+--       cases hprot; grind
+--     | pinit2 =>
+--       cases hprot; grind
+--     | part2 =>
+--       cases hprot; grind
+--     | part1 =>
+--       cases hprot; specialize @ih b
+--       dsimp [PState.consistentWith] at *
+--       rename_i a
+--       rw [a] at ih ⊢; dsimp at *
+
+--     | commit =>
+--       cases hprot; specialize @ih true; grind
+--     | abort =>
+--       cases hprot; specialize @ih true; grind
+
+-- theorem comm_part1_commit {s s' s''} (hphi : φ s) :
+--   Protocol .part1 s s' →
+--   Protocol .commit s s'' →
+--   Protocol .commit s' s'' := by
+--   induction hphi generalizing s' s'' with
+--   | base_commit => sorry
+--   | base_abort => sorry
+--   | @step s_p s'_p r hphi' hprot ih =>
+--     intro htrans1 htrans2
+--     cases r with
+--     | pinit1 =>
+--       obtain ⟨s_pinit_comm, h_pinit, h_comm⟩ := comm_pinit1_commit ‹_› ‹_›
+--       obtain ⟨s_pinit_part1, h_pinit2, h_part1⟩ := comm_pinit1_part1 hprot ‹_›
+--       have : Protocol Rule.commit s_pinit_part1 s_pinit_comm := by grind
+--       sorry
+--     | pinit2 =>
+--       sorry
+--     | part2 =>
+--       sorry
+--     | part1 =>
+--       have : s'_p = s' := by grind [part1_det]
+--       subst_vars
+--       apply ih; grind [part1_twice]
+--       skip
+--     | commit => sorry
+--     | abort => sorry
+
+-- theorem comm_part2_commit {s s' s''} :
+--   Protocol .part2 s s' →
+--   Protocol .commit s s'' →
+--   ∃ s''', Protocol .part2 s'' s''' ∧ Protocol .commit s' s''' := by
+--   -- Commit makes p2 committed, disabling the part2 step on that branch.
+--   sorry
+
+-- --miss all the abort cases right?
 
 end TwoPhaseCommit
+end THEORY
